A **series** is just the sum of terms of a [[Maths/Calc 2/8. Sequences and Series#^b8564d|Sequences]].

Let $a_{n} = (\frac{1}{2})^{n}$ for $n \geq 1$
a) $a_{1}+a_{2}+a_{3}=\frac{1}{2} + \frac{1}{4} + \frac{1}{8}=\frac{7}{8}$
b) $a_{1} + a_{2} + a_{3} \dots a_{6} = \frac{1}{2} + \frac{1}{4} + \frac{1}{8} \dots + \frac{1}{64} = \frac{63}{64}$
c) The partial sums, would be $S_{N} = \frac{2^{N} - 1}{2^{N}}$
d) Seems like the more terms you add to this sequence, the closer you get to the number $1$. Hence, it makes sense to find $\displaystyle \sum_{n=1}^{\infty} a_{n}= \lim_{N \to \infty} \frac{2^{N} - 1}{2^{N}} = 1$.

Moreover, given an infinite sequence $\set{a_n}_{n \geq 1}$, an expression of form $a_{1}+a_{2}+a_{3}+\dots$ is called an **infinite series** and is written $\displaystyle \sum_{n=1}^{\infty} a_n$

Given an infinite series, $\displaystyle \sum_{n=1}^{\infty} a_n$, we define it's sequence of partial sums to be $\set{S_N}_{N \geq 1}$ where $S_{N} = a_{1} + a_{2} + a_{3} + \dots a_{N}$ i.e. $\displaystyle \sum_{n=1}^{N} a_n$

If the partial sums converge to a single, finite number, the infinite series converges.

---
Given an infinite series $\displaystyle \sum^{\infty}_{n=1} a_{n}$
There are two associated sequences:
- Sequence of terms of series 
	$a_1,a_2,a_3,\dots$
- Sequence of partial sums
	$(a_1),(a_1+a_2),(a_1+a_2+a_3),\dots$

Note the distinction between the two!
The Infinite series $\displaystyle \sum^{\infty}_{n=1} a_{n}= \lim_{N \to \infty} S_N$
i.e. it is what the Sequence of partial sums approach and NOT the terms themselves.

However, it is hard to do that. So we come with niche ways to connect the simpler to study Sequence of terms with that of the Partial Sums to make a guess about what the infinite Series does. ^04f8a2

---
### Geometric Series 
A **Geometric Series** is a series whose terms form a geometric sequence
	$\displaystyle \sum^{\infty}_{n=k} ar^n$
What we want to know is when does a geometric series converges and if it does, what does it converge to?

Let's find a formula for the partial sums of a geometric series.
$\displaystyle S_{N} = \sum^{N}_{n=k} ar^{n} = ar^{k} + ar^{k+1} + ar^{k+2} + \dots ar^{N-1} + ar^{N}$
To find a helpful formula for $S_{N}$, we can find instead
		$rS_{N} = \quad \quad ar^{k+1} + ar^{k+2} + ar^{k+3} +\dots  ar^{N} + ar^{N+1}$
But because of so many common terms, we can subtract the two equations and we will only be left with 2 terms (the first and the last)

$S_{N} - rS_{N} = ar^{k} - ar^{N+1}$
$\implies S_{N} (1-r) = ar^{k}(1-r^{N+1-k})$
$$\implies S_{N} = \frac{ar^{k}(1-r^{N+1-k})}{1-r}$$
Hence, $\displaystyle \lim_{N \to \infty} S_{N} = \lim_{N \to \infty} \frac{ar^{k}(1-r^{N+1-k})}{1-r} = \cases{\frac{ar^{k}}{1-r}, \space |r|<1 \\ diverges, \space |r| > 1 \\ diverges, \space r=-1}$ 

The if $|r|<1$, the $r^{N+1-k}$ goes to 0 as $N \to \infty$. Hence the geometric sum itself converges.
If $|r| > 1$, the term goes to infinity and hence the geometric sum diverges.
Even at $r=-1$, the term oscillates and because $|r|=1$, the oscillation never settles to some unique value. (For $r=1$, you're adding the same number infinite times and hence, it again diverges unless $a=0$).

Hence, a geometric sum (Geometric series) only converges if the ratio between numbers has a magnitude $<1$, in which case it is $\frac{ar^{k}}{1-r}$.

Note, this is when you sum from $n=k$ to $n=\infty$

The $a(\frac{1-r^{N}}{1-r})$ is true for the sum of **N terms starting from $n=0$**
That means that $\sum^{n=N-1}_{n=0}a_{n}$ This is NOT a general form.

For $\sum^{n=N}_{n=0}a_{n}$ you would have $a(\frac{1-r^{N+1}}{1-r})$

You can use the form to derive the general expression by setting $\sum^{N}_{k}a_{n}=\sum^{N}_{0}a_{n} - \sum^{k-1}_{0} a_{n} = a(\frac{1-r^{N+1}}{1-r})-a(\frac{1-r^{k}}{1-r})=\frac{ar^{k}(1-r^{N+1-k})}{1-r}$

The limiting sum would have the terms inside the parenthesis being simply 1. Hence, $S_{\infty} = \frac{ar^{k}}{1-r}$

**THERE IS NOT JUST THE EXPONENT WITHIN THE PARENTHESIS THAT CHANGES BUT ALSO THE $r^k$ TERM OUTSIDE THE PARENTHESIS!!! ALWAYS DERIVE THIS! NEVER MEMORIZE.**


---
#### Examples 
$\sum^{\infty}_{n=0}4 (\frac{-2}{3})^n$ converges ($\frac{|-2|}{3}< 1$) and converges to $\frac{4}{(1-(\frac{-2}{3}))}$

$\sum^{\infty}_{n=0} 6(\frac{4}{7})^{2n}$ also converges. **NOTE**, to write the sum, you need a form $ar^{n}$ hence you want to write this as $6 \cdot ((\frac{4}{7})^{2})^{n}$ hence $a=6$ and $r=\frac{16}{49}$ hence $\frac{ar^{k}}{1-r} = \frac{6*16^{2}}{49*33}$


---
### Telescoping Series 
$\displaystyle \sum^{\infty}_{n=1} \frac{1}{\sqrt{n+1}} - \frac{1}{\sqrt{n}}$

$S_{1} = \frac{1}{\sqrt{2}}- \frac{1}{\sqrt{1}}$
$S_{2} = \frac{1}{\sqrt{2}}- \frac{1}{\sqrt{1}} + \frac{1}{\sqrt{3}}- \frac{1}{\sqrt{2}} = \frac{1}{\sqrt{3}} - \frac{1}{\sqrt{1}}$
$S_{3} = S_{2} + \frac{1}{\sqrt{4}}- \frac{1}{\sqrt{3}} = \frac{1}{\sqrt{3}} - \frac{1}{\sqrt{1}} + \frac{1}{\sqrt{4}}- \frac{1}{\sqrt{3}} = \frac{1}{\sqrt{4}}- \frac{1}{\sqrt{1}}$
Hence, in general, $S_{n} = \frac{1}{\sqrt{n+1}} - \frac{1}{\sqrt{1}}$
Hence, $S_{\infty} = \frac{1}{\sqrt{\infty+1}} - 1 = -1$

This idea is called telescoping since you collapse the end terms as if collapsing an extended form of a telescope into just the eyepiece and the lens.

You usually have to try things out and get your hands dirty while playing around with them but a nice indicator or a telescoping series, you might see **terms that subtract** but are **offset from one another**.
But again, often, terms only start cancelling out once you are further down expanding the series so DO NOT rely on these indicators alone.

As Prof. Stone says,
>Maths is often more of an art than a science, and you just have to realize things.

![[Maths/Calc 2/attachments/2024_10_16 6_46 pm Office Lens.jpg|400]]

---

Again, back to [[#^04f8a2|what we thought above]], it's kinda hard to find an actual formula for the terms of the sequence of the Sums $S_{N}$ itself.

Can we find insights with the terms $a_{n}$
 themselves?

## The Divergence Test
#theorem If $\sum a_{n}$ converges, then $\displaystyle \lim_{n \to \infty} a_{n}=0$ 
* Corollary
**nth term Test for Divergence**
If $\lim_{n \to \infty} a_{n} \neq 0$, then $\sum a_{n}$ diverges 

Does $\sum^{\infty}_{n=1} (1 - \frac{1}{n})^{n}$ converge? No! Because $\lim_{n \to \infty} (1 - \frac{1}{n})^{n} = \frac{1}{e}$ (there's a $-$ve sign so all terms are at least $\frac{1}{e}$ hence adding them infinitely would end up booming to infinity)

---
a) Find $\lim_{n \to \infty} n \, tan(\frac{1}{n})$
	$= \lim_{n \to \infty} \frac{sin(\frac{1}{n})}{\frac{1}{n} \cdot cos(\frac{1}{n})}$
	$= \lim_{h \to 0} \frac{sin(h)}{h} \cdot \frac{1}{cos(h)}$
	$=1$
Hence the series diverges since the terms themselves never approach 0.

Remember! If the terms never converge to 0, the sum can never do!

As a converse of this, Just because the terms approach 0 it does NOT mean the sum must too! Example, $a_{n} = \frac{1}{n}$ has terms converging to 0 but the series doesn't converge to a value.

