
#def Curve 
A curve is a function that maps some variable (such as $t$) to a point in some space such as $(x,y,z)$.

$\vec{r}(t) = (x(t), y(t), z(t))$

---
![[Maths/Multivariable Calc/attachments/Drawing 25-02-17-03-56-05]]

Note, the way you represent for instance a cylinder is the following...
Irrespective of the $z$ value, you create a curve for a slice parallel to the $x-y$ plane.

Hence, the cylinder from $-z_{0}$ to $z_{0}$ would be $x^2+y^2=r^2\,\{-z_0<z<z_0\}$

A plane, like an extension to say a point in 1 dimension ($a=c$), a line in 2 dimensions $ax+by=c$, is a lower dimensional object in $3$ dimensions

Hence, it is $ax+by+cz=d$

To find the curve that the plane slices through the surface, just simultaneously solve the system of equations formed by both the equations of the surfaces. (You can use whatever method you want - elimination/substitution)

---

Note, a defining feature of a plan is its normal vector.
The normal vector for any plane $ax+by+cz=d$ would be literally $\vec{n} = (a\hat{i}, b\hat{j}, c\hat{k})$

(Note, this isn't a unit normal, for that you will have to normalize this.
In fact, this normal vector is not "THE" unit vector but just "A" unit vector)

The reason for this is the normal is literally just any cross product between any two points of the plane.

---
### Tangent Lines and Slopes for multidimensional functions

The Slope of a function $f'(x) = \lim_{\Delta x \to 0} \frac{f(x+\Delta x) - f(x)}{\Delta x}$

similarly, since the derivative $\frac{d}{dx}(g(x) + f(x)) = \frac{d}{dx}(g(x)) + \frac{d}{dx}(f(x))$

>Thus derivative of a sum of functions is the sum of derivatives of the functions
>i.e. the derivative is a linear operator

For $\vec{r}(t) = (x,y,z)$
$\frac{d\vec{r}}{dt} = (\frac{dx}{dt} + \frac{dy}{dt} + \frac{dz}{dt})$ ^40883f

Essentially, for a higher dimensional function, the derivative has a component from each orthogonal component for which the components are independently defined from each other for the given parameterization.

---
Note, for a different parameterization $u$, $\frac{d\vec{r}}{dt} = \frac{d\vec{r}}{du} \frac{du}{dt}$
(By the chain rule... beware of the Math Police for any reasoning for using fractions.)

You can stack higher order derivatives such as $\ddot{r} = (\ddot{x}, \ddot{y}, \ddot{z})$ (given that the orthogonal components are independent of each other for the given parameterization)

(here, $\ddot{a} = \frac{d^{2}a}{dt^{2}}$)

---
Take our initial example of a cylinder ($x^{2}+ y^{2}=2$) sliced by the curve $x+2y+z=4$.

It'll create some sort of an ellipse-like shape in 3 dimensions.

What would be the tangent line at $(1,1,1)$? (Given, and verifiable that the point lies on the curve of the intersection)

$l = \vec{P} + \lambda \vec{D}$
So the question is for finding the direction vector of the tangent line (and hence the gradient!) since we already have a point $\vec{P} = (1,1,1)$


Solving the equations simultaneously, you first parameterize one of the functions

You can parameterize the cylinder simply by 
$x=rcos(\theta)$ and $y=rsin(\theta)$
$\implies x=\sqrt{2}cos(t)$ and $y = \sqrt{2}sin(t)$

Now you can plug in this value in the second curve to parameterize the only remaining variable ($z$)

$x+2y+z=4 = \sqrt{2}cos(t) + 2\sqrt{2}sin(t)+z=4$
Hence, $z = 4 - \sqrt{2}cos(t) - 2\sqrt{2}sin(t)$

Hence, the curve 
$$\vec{r}(t) = (\sqrt{2}cos(t), \sqrt{2}sin(t), 4 - \sqrt{2}cos(t) - 2\sqrt{2}sin(t))$$
Now the gradient $\frac{d\vec{r}}{dt} = (\frac{dx}{dt}, \frac{dy}{dt}, \frac{dz}{dt}) = (-\sqrt{2}sin(t), \sqrt{2}cos(t), \sqrt{2}sin(t) - 2\sqrt{2}cos(t))$

To find the gradient at $(1,1,1)$, we need to find what value of $t$ corresponds to the given point.

We know $\sqrt{2}cos(t) = 1 \implies t = \frac{\pi}{4}$
(This should be an obvious solution)

Hence, the tangent = $(-\sqrt{2}sin(\frac{\pi}{4}), \sqrt{2}cos(\frac{\pi}{4}), \sqrt{2}sin(\frac{\pi}{4}) - 2\sqrt{2}cos(\frac{\pi}{4}))$

$\frac{d\vec{r}}{dt}=\vec{v} = (-1,1,-1)$

Hence, the tangent line $\vec{P} + \lambda \vec{D} = (1,1,1) + \lambda (-1,1,-1)$

---
An interesting thing to note would be that in 3 dimensions, tangent to a point at a surface would be a PLANE instead of a line.

Hence, for both the surfaces (the cylinder and the plane), you would get 1 plane each. The line of intersections of those planes, in fact, would be the tangent line.

In essence, the line of tangency is tangent to both the surfaces which give rise to the curve of intersection (it has to be)!

---
### Product Rule
A nice fact to leverage here is $\frac{d}{dx}(f(x)g(x)) = \frac{df}{dx}g(x) + f(x) \frac{dg}{dx}$

Product rule for dot product:
$\frac{d}{dt}(\vec{u_{1}}(t) \cdot \vec{u_{1}}(t)) = \frac{d\vec{u_{1}}}{dt} \cdot \vec{u_{2}}(t) + \vec{u_{1}}(t) \cdot \frac{d\vec{u_{2}}}{dt}$

(essentially the same but you have to remember the kind of multiplication you are doing)

---
#### Application of the Derivative of the Product rule for dot products
![[Maths/Multivariable Calc/attachments/Drawing 25-02-17-04-47-02]]
Let's say a particle of mass $m$ traces out a path.

The kinetic energy $\frac{1}{2}mv^{2} = \frac{1}{2}m( \vec{v(t)} \cdot \vec{v(t)})$
(remember... $\vec{a} \cdot \vec{a} = a^{2}$)

Say you want to know the rate of change of your kinetic energy...
You would have to say $\frac{d}{dt}(KE) = \frac{d}{dt}(\frac{1}{2}m(\vec{v}(t) \cdot \vec{v}(t)))$
$= \frac{1}{2}m (\frac{d\vec{v}}{dt}\cdot\vec{v}(t) + \vec{v}(t) \cdot \frac{d\vec{v}}{dt})$
$= \frac{1}{2}m(2 \frac{d\vec{v}}{dt} \cdot \vec{v}(t))$
$= m \vec{a}(t) \cdot \vec{v}(t)$
Hence, $\frac{dK}{dt} = \vec{F}(t) \cdot \vec{v}(t)$ (that is $\frac{dK}{dt} = Power = \frac{Work}{time}$!)

Hence, $\Delta K = \int \vec{F}(t) \cdot \vec{v}(t) \, dt$
Hence, you prove that Work Done is the change in Kinetic Energy! 
(The work energy theorem!)

---
### Product Rule for cross product
$\frac{d}{dt}(\vec{u_{1}}(t) \times \vec{u_{1}}(t)) = \frac{d\vec{u_{1}}}{dt} \times \vec{u_{2}}(t) + \vec{u_{1}}(t) \times \frac{d\vec{u_{2}}}{dt}$

NOTE! The order matters!

So when crossed, do not switch the respective orders of the terms in the product!

A simple application would be
$\vec{L}(t) = \text{angular momentum} = m (\vec{r}(t) \times \vec{v}(t))$

Hence, you can see that the time derivative of the angular momentum would be $\frac{d\vec{L}}{dt} = m(\frac{d\vec{r}}{dt} \times \vec{v}(t) + \vec{r}(t) \times \frac{d\vec{v}}{dt})$
$\implies \frac{d\vec{L}}{dt} = m(\vec{v}(t) \times \vec{v}(t) + \vec{r}(t) \times \vec{a}(t))$
And since $\vec{a} \times \vec{a} = \vec{0}$

$\frac{d\vec{L}}{dt} = m(\vec{r}(t) \times \vec{a}(t)) = \vec{r}(t) \times m\vec{a}(t) = \vec{r}(t) \times \vec{F}(t)$

Ahaa! Hence, $\frac{d\vec{L}}{dt} = \vec{\tau}(t)$

A very nice implication of this is that for a system of masses like the sun and the Earth... Since gravity is a central force ![[Maths/Multivariable Calc/attachments/Drawing 25-02-17-05-02-25]]
Hence, the gravitational force applies no Torque on the Earth. Hence, angular momentum of the Earth (or any planet for that matter) is conserved!

$\vec{L}(t) = \text{angular momentum} = m (\vec{r}(t) \times \vec{v}(t))$

But the angular momentum is related to a cross product and hence an area (remember, the cross product is just an area vector!). Hence some sort of area must be conserved.

That is the Kepler's Kaw of Equal Areas being traversed in equal times!


---

Essentially the idea is that the product rule works for all products, given you remember and apply the same product throughout.




